Prove that step/steps preserve the consistency of the state

src/metaproperties.v
@@ -34,6 +34,8 @@ Ltac case_analysis H :=
 (* Misc *)
 
 Definition consistent_state (s : State) :=
+  (forall ctr, In ctr (m_contracts s) -> m_fresh_id s > ctr_id ctr) /\
+  (forall c_id, (In (Executed c_id) (m_events s) \/ In (Deleted c_id) (m_events s)) -> m_fresh_id s > c_id) /\
   (forall ctr ctr', In ctr (m_contracts s) -> In ctr' (m_contracts s) -> (ctr_id ctr = ctr_id ctr') -> ctr = ctr') /\
   (forall ctr, In ctr (m_contracts s) -> (~ In (Executed (ctr_id ctr)) (m_events s) /\ ~ In (Deleted (ctr_id ctr)) (m_events s))) /\
   (forall e, ~ (In (Executed e) (m_events s) /\ In (Deleted e) (m_events s))).
@@ -196,7 +198,7 @@ Qed.
 
 
 (* step does not remove transactions from the ledger *)
-Lemma steps_does_not_remove_transactions:
+Theorem steps_does_not_remove_transactions:
   forall tr s1 s2,
     steps s1 s2 ->
     In tr (m_ledger s1)->
@@ -211,22 +213,351 @@ Proof.
   trivial.
 Qed.
 
+Lemma rm_in:
+  forall cs c, In c (rm c cs) -> False.
+Proof.
+  induction cs; intros; simpl in *; try contradiction.
+  case_eq (ctr_eq_dec c a); intros H0 H'; rewrite H' in H; try contradiction.
+  subst c. eapply IHcs; eauto.
+Qed.
 
-(* Metaproperties about events *)
-Axiom step_preserves_consistent_state:
+
+Lemma execute_produces_new_ids:
+  forall P sc I O bal time gtw c_id dsc_id bal' ctrs' next_id' L' next_id L,
+    execute P sc I O bal  time gtw c_id dsc_id next_id L = Some (result bal' ctrs' next_id' L') ->
+    next_id' >= next_id.
+Proof.
+  intros P. induction P; intros; simpl in H; inversion H; clear H.
+  - omega.
+  - omega.
+  - eapply IHP; eauto.
+  - case_match H1.
+    eapply IHP; eauto.
+  - eapply IHP; eauto.
+  - case_match H1. destruct r.
+    case_match H2. destruct r.
+    inversion H3. clear H3.
+    subst ctrs'.
+    apply IHP1 in H.
+    apply IHP2 in H0.
+    subst. omega.
+  - subst. omega.
+  - case_match H1.
+    case_eq (n =? 0); intros H0; rewrite H0 in H2.
+    + eapply IHP2; eauto.
+    + eapply IHP1; eauto.
+  - case_if H1.
+    case_if H2.
+    + eapply IHP; eauto.
+    + subst. omega.
+Qed.
+
+
+Lemma step_preserves_consistent_state_1:
+  forall s s',
+    step s s' ->
+    consistent_state s ->
+    (forall ctr : FinContract,
+        In ctr (m_contracts s') -> m_fresh_id s' > ctr_id ctr).
+Proof.
+  intros.
+  destruct H0 as [H0 [He [H' [T P]]]].
+  induction H; subst s'; simpl in *; auto.
+  - destruct H1 as [H1 | H1].
+    + subst. simpl in *. omega.
+    + apply H0 in H1. omega.
+  - case_eq (ctr_eq_dec ctr ctr0); intros; try contradiction.
+    subst ctr0.
+    apply in_app_iff in H1.
+    destruct H1 as [H1 | H1].
+    + exfalso. eapply rm_in. exact H1.
+    + apply execute_produces_new_ids in H7.
+      apply H0 in H.
+      omega.
+  - case_eq (ctr_eq_dec ctr ctr0); intros; try contradiction.
+    subst ctr0.
+    apply in_app_iff in H1.
+    destruct H1 as [H1 | H1].
+    + exfalso. eapply rm_in. exact H1.
+    + apply execute_produces_new_ids in H7.
+      apply H0 in H.
+      omega.
+  - case_eq (ctr_eq_dec ctr ctr0); intros; try contradiction.
+    subst ctr0.
+    apply in_app_iff in H1.
+    destruct H1 as [H1 | H1].
+    + exfalso. eapply rm_in. exact H1.
+    + apply execute_produces_new_ids in H7.
+      apply H0 in H.
+      omega.
+  - case_eq (ctr_eq_dec ctr ctr0); intros; try contradiction.
+    subst ctr0. auto.
+Qed.
+
+
+Lemma step_preserves_consistent_state_2:
+  forall s s',
+    step s s' ->
+    consistent_state s ->
+    (forall c_id : Id,
+        In (Executed c_id) (m_events s') \/ In (Deleted c_id) (m_events s') ->
+        m_fresh_id s' > c_id).
+  intros.
+  destruct H0 as [H0 [He [H' [T P]]]].
+  induction H; subst s'; simpl in *; auto.
+  - destruct H1 as [[H1 | H1] | [H1 | H1]]; try inversion H1; assert (H'' : m_fresh_id s > c_id); auto.
+  - destruct H1 as [[H1 | H1] | [H1 | H1]]; try inversion H1; subst.
+    + apply execute_produces_new_ids in H7; apply H0 in H. omega.
+    + apply execute_produces_new_ids in H7.
+      assert (H'' : m_fresh_id s > c_id); auto.
+      omega.
+    + apply execute_produces_new_ids in H7.
+      assert (H'' : m_fresh_id s > c_id); auto.
+      omega.
+  - destruct H1 as [[H1 | H1] | [H1 | H1]]; try inversion H1; subst.
+    + apply execute_produces_new_ids in H7; apply H0 in H. omega.
+    + apply execute_produces_new_ids in H7.
+      assert (H'' : m_fresh_id s > c_id); auto.
+      omega.
+    + apply execute_produces_new_ids in H7.
+      assert (H'' : m_fresh_id s > c_id); auto.
+      omega.
+  - destruct H1 as [[H1 | H1] | [H1 | H1]]; try inversion H1; subst.
+    + apply execute_produces_new_ids in H7; apply H0 in H. omega.
+    + apply execute_produces_new_ids in H7.
+      assert (H'' : m_fresh_id s > c_id); auto.
+      omega.
+    + apply execute_produces_new_ids in H7.
+      assert (H'' : m_fresh_id s > c_id); auto.
+      omega.
+  - apply H0 in H. 
+    destruct H1 as [[H1 | H1] | [H1 | H1]]; try inversion H1; subst; auto.
+Qed.
+
+
+Ltac case_eq_dec_ctr c1 c2 c :=
+  case_eq (ctr_eq_dec c1 c); intros; try contradiction;
+  case_eq (ctr_eq_dec c2 c); intros; try contradiction;
+  subst c1 c2; trivial.
+
+Lemma step_preserves_consistent_state_3:
+  forall s s',
+    step s s' ->
+    consistent_state s ->
+    forall ctr ctr' : FinContract,
+       In ctr (m_contracts s') ->
+       In ctr' (m_contracts s') ->
+       ctr_id ctr = ctr_id ctr' -> ctr = ctr'.
+Proof.
+  intros.
+  destruct H0 as [H0 [He [H' [T P]]]].
+  induction H; subst s'; simpl in *; try case_eq_dec_ctr ctr ctr' ctr0.
+  - case_eq_dec_ctr ctr ctr' new_contract.
+  - apply H'; auto.
+Qed.
+
+Ltac contradict_unfold :=
+  let He := fresh "H" in
+  unfold not; split; intros He; destruct He as [He | He]; try inversion He.
+
+
+Lemma execute_produces_new_contracts:
+  forall P sc I O bal time gtw c_id
+         dsc_id bal' ctrs' next_id' L' next_id L,
+    execute P sc I O bal  time gtw c_id dsc_id next_id L =
+    Some (result bal' ctrs' next_id' L') ->
+    next_id > c_id ->
+    forall ctr', In ctr' ctrs' -> (ctr_id ctr') <> c_id.
+Proof.
+  intros P.
+  induction P; intros* H; intros; simpl in H; inversion H; clear H.
+  - subst. contradiction.
+  - subst. contradiction.
+  - eapply IHP; eauto.
+  - case_match H2.
+    eapply IHP; eauto.
+  - eapply IHP; eauto.
+  - case_match H2.
+    destruct r.
+    case_match H3.
+    destruct r.
+    inversion H5. clear H5. subst ctrs'.
+    simpl in H1.
+    apply in_app_iff in H1.
+    destruct H1 as [H1 | H1].
+    + eapply IHP1; eauto.
+    + eapply IHP2; eauto.
+      apply execute_produces_new_ids in H.
+      apply execute_produces_new_ids in H2.
+      subst. omega.
+  - subst ctrs'. simpl in *.
+    destruct H1 as [H1 | H1]; auto.
+    subst. simpl. omega.
+  - case_match H3.
+    case_if H4.
+    + eapply IHP2; eauto.
+    + eapply IHP1; eauto.
+  - case_if H3.
+    case_if H4.
+    + eapply IHP; eauto.
+    + subst. simpl in *.
+      destruct H1 as [H1 | H1]; try contradiction.
+      subst. simpl in *.
+      omega.
+Qed.
+
+
+Lemma step_preserves_consistent_state_4:
+  forall s s',
+    step s s' ->
+    consistent_state s ->
+    (forall ctr,
+        In ctr (m_contracts s') ->
+        (~ In (Executed (ctr_id ctr)) (m_events s') /\
+         ~ In (Deleted (ctr_id ctr)) (m_events s'))).
+Proof.
+  intros.
+  destruct H0 as [H' [He [H0 [T P]]]].
+  induction H; subst s'; simpl in *.
+  - contradict_unfold.
+    destruct H1 as [H1 | H1].
+    + subst ctr new_contract. simpl in *.
+      assert (Hf: m_fresh_id s > m_fresh_id s).
+      apply He; left. trivial.
+      omega.
+    + apply T in H1. destruct H1 as [H1 _]. contradiction.
+    + destruct H1 as [H1 | H1].
+      ++ subst ctr new_contract. simpl in *.
+         assert (Hf: m_fresh_id s > m_fresh_id s).
+         apply He; right. trivial.
+         omega.
+      ++ apply T in H1. destruct H1 as [_ H1]. contradiction.
+  - case_eq (ctr_eq_dec ctr ctr0); intros; try contradiction.
+    subst ctr0.
+    unfold not; split; intros.
+    + destruct H9 as [H9 | H9]; try contradiction.
+      apply in_app_iff in H1.
+      destruct H1 as [H1 | H1].
+      ++ eapply rm_in. exact H1.
+      ++ unfold exec_ctr_in_state_with_owner in H7.
+         apply execute_produces_new_contracts with (ctr' := ctr) in H7; try contradiction.
+         apply H'; auto.
+         trivial.
+    + destruct H9 as [H9 | H9]; try inversion H9.
+      apply T in H.
+      destruct H as [_ H]; try contradiction.
+  - case_eq (ctr_eq_dec ctr ctr0); intros; try contradiction.
+    subst ctr0.
+    unfold not; split; intros.
+    + destruct H9 as [ | H9].
+      apply in_app_iff in H1.
+      destruct H1 as [H1 | H1].
+      ++ eapply rm_in. exact H1.
+      ++ unfold exec_prim_ctr_in_state_with_owner in H7.
+         apply execute_produces_new_contracts with (ctr' := ctr) in H7; try contradiction.
+         apply H'; auto.
+         trivial.
+      ++  unfold exec_prim_ctr_in_state_with_owner in H7.
+          apply execute_produces_new_contracts with (ctr' := ctr) in H7; try contradiction.
+    + destruct H9 as [H9 | H9]; try inversion H9.
+      apply T in H.
+      destruct H as [_ H]; try contradiction.
+  - case_eq (ctr_eq_dec ctr ctr0); intros; try contradiction.
+    subst ctr0.
+    unfold not; split; intros.
+    + destruct H9 as [ | H9].
+      apply in_app_iff in H1.
+      destruct H1 as [H1 | H1].
+      ++ eapply rm_in. exact H1.
+      ++ unfold exec_prim_ctr_in_state_with_owner in H7.
+         apply execute_produces_new_contracts with (ctr' := ctr) in H7; try contradiction.
+         apply H'; auto.
+         trivial.
+      ++  unfold exec_prim_ctr_in_state_with_owner in H7.
+          apply execute_produces_new_contracts with (ctr' := ctr) in H7; try contradiction.
+    + destruct H9 as [H9 | H9]; try inversion H9.
+      apply T in H.
+      destruct H as [_ H]; try contradiction.
+  - case_eq (ctr_eq_dec ctr ctr0); intros; try contradiction.
+    subst ctr0.
+    split; unfold not; intros; eapply rm_in; eauto.
+  - apply T; auto.
+Qed.
+
+
+Lemma step_preserves_consistent_state_5:
+  forall s s',
+    step s s' ->
+    consistent_state s ->
+    (forall e : Id,
+        ~ (In (Executed e) (m_events s') /\ In (Deleted e) (m_events s'))).
+Proof.
+  intros.
+  destruct H0 as [H' [He [H0 [T P]]]].
+  induction H; subst s'; simpl in *; auto; unfold not; intros C.
+  - destruct C as [[C | C'] [D | D']];
+      try inversion C; try inversion D.
+    unfold not in P. eapply P; eauto.
+  - destruct C as [[C | C'] [D | D']];
+      try inversion C; try inversion D.
+    + apply T in H.
+      destruct H as [_ H].
+      subst. contradiction.
+    + unfold not in P. eapply P; eauto.
+  - destruct C as [[C | C'] [D | D']];
+      try inversion C; try inversion D.
+    + apply T in H.
+      destruct H as [_ H].
+      subst. contradiction.
+    + unfold not in P. eapply P; eauto.
+  - destruct C as [[C | C'] [D | D']];
+      try inversion C; try inversion D.
+    + apply T in H.
+      destruct H as [_ H].
+      subst. contradiction.
+    + unfold not in P. eapply P; eauto.
+  - destruct C as [[C | C'] [D | D']];
+      try inversion C; try inversion D.
+    + apply T in H.
+      destruct H as [H _].
+      subst. contradiction.
+    + unfold not in P. eapply P; eauto.
+Qed.
+
+
+Theorem step_preserves_consistent_state:
   forall s s',
     step s s' ->
     consistent_state s ->
     consistent_state s'.
+Proof.
+  intros.
+  unfold consistent_state.
+  split.
+  - eapply step_preserves_consistent_state_1; eauto.
+  - split.
+    + eapply step_preserves_consistent_state_2; eauto.
+    + split.
+      ++ eapply step_preserves_consistent_state_3; eauto.
+      ++ split.
+         ** eapply step_preserves_consistent_state_4; eauto.
+         ** eapply step_preserves_consistent_state_5; eauto.
+Qed.
 
-Axiom steps_preserves_consistent_state:
+
+Theorem steps_preserves_consistent_state:
   forall s s',
     steps s s' ->
     consistent_state s ->
     consistent_state s'.
+Proof.
+  intros.
+  induction H; subst; auto.
+  eapply step_preserves_consistent_state; eauto.
+Qed.
 
 
-Lemma events_consistent_step:
+Theorem events_consistent_step:
   forall s s' e,
     step s s' ->
     In e (m_events s) ->
@@ -285,7 +616,7 @@ Qed.
 (* Metaproperties about contract execution *)
 
 
-Lemma step_effect_over_contract:
+Theorem step_effect_over_contract:
   forall ctr s s',
     step s s' ->
     In ctr (m_contracts s) ->
@@ -314,7 +645,7 @@ Proof.
   - subst s'. simpl. left. trivial.
 Qed.
 
-Lemma steps_effect_over_contract:
+Theorem steps_effect_over_contract:
   forall ctr s s',
     steps s s' ->
     In ctr (m_contracts s) ->
@@ -396,7 +727,7 @@ Proof.
 Qed.
 
 
-Lemma step_executes_only_one_contract:
+Theorem step_executes_only_one_contract:
   forall ctr ctr' s s',
     step s s' ->
     consistent_state s ->
@@ -407,18 +738,18 @@ Lemma step_executes_only_one_contract:
     ctr = ctr'.
 Proof.
  intros *. intros H. induction H; intros; subst s'; unfold consistent_state in *.
- - destruct H5 as [H' [T P]].
+ - destruct H5 as [O [A [H' [T P]]]].
    simpl in H8, H9.
    destruct H8 as [H8 | H8]; try inversion H8.
    destruct H9 as [H9 | H9]; try inversion H9.
    apply T in H8; auto; try contradiction.
  - simpl in H10, H11.
    destruct H10 as [H10 | H10]; try inversion H10.
-   destruct H7 as [H' [T P]].
+   destruct H7 as  [O [A [H' [T P]]]].
    destruct H11 as [H11 | H11]; try inversion H11.
    + rewrite H7 in H12. apply H'; auto.
    + apply T in H9. destruct H9 as [H9 _]; contradiction.
-   + destruct H7 as [H' [T P]].
+   + destruct H7 as  [O [A [H' [T P]]]].
      destruct H11 as [H11 | H11]; try inversion H11.
      * apply T in H8.
        destruct H8 as [H8 _]; contradiction.
@@ -426,11 +757,11 @@ Proof.
        destruct H8 as [H8 _]; contradiction.
  - simpl in H10, H11.
    destruct H10 as [H10 | H10]; try inversion H10.
-   destruct H7 as [H' [T P]].
+   destruct H7 as [O [A [H' [T P]]]].
    destruct H11 as [H11 | H11]; try inversion H11.
    + rewrite H7 in H12. apply H'; auto.
    + apply T in H9. destruct H9 as [H9 _]; contradiction.
-   + destruct H7 as [H' [T P]].
+   + destruct H7 as [O [A [H' [T P]]]].
      destruct H11 as [H11 | H11]; try inversion H11.
      * apply T in H8.
        destruct H8 as [H8 _]; contradiction.
@@ -438,11 +769,11 @@ Proof.
        destruct H8 as [H8 _]; contradiction.
  - simpl in H10, H11.
    destruct H10 as [H10 | H10]; try inversion H10.
-   destruct H7 as [H' [T P]].
+   destruct H7 as [O [A [H' [T P]]]].
    destruct H11 as [H11 | H11]; try inversion H11.
    + rewrite H7 in H12. apply H'; auto.
    + apply T in H9. destruct H9 as [H9 _]; contradiction.
-   + destruct H7 as [H' [T P]].
+   + destruct H7 as [O [A [H' [T P]]]].
      destruct H11 as [H11 | H11]; try inversion H11.
      * apply T in H8.
        destruct H8 as [H8 _]; contradiction.
@@ -451,15 +782,15 @@ Proof.
  - simpl in H8, H9.
    destruct H8 as [H8 | H8]; try inversion H8.
    destruct H9 as [H9 | H9]; try inversion H9.
-   destruct H5 as [H' [T P]].
+   destruct H5 as [O [A [H' [T P]]]].
    apply T in H8; auto; try contradiction.
  - simpl in H3, H4.
-   destruct H0 as [H' [T P]].
+   destruct H0 as [O [A [H' [T P]]]].
    apply T in H3; auto; try contradiction.
 Qed.
 
 
-Lemma step_does_not_remove_events:
+Theorem step_does_not_remove_events:
   forall s s' e,
     step s s' ->
     In e (m_events s) ->
